permission_bits_separation.v
@@ -1,6 +1,6 @@
 (* Copyright (c) 2012-2014, Robbert Krebbers. *)
 (* This file is distributed under the terms of the BSD license. *)
-Require Export permission_bits.
+Require Export permission_bits_refine.
 
 Section permission_bits.
 Context `{EnvSpec Ti}.
@@ -12,6 +12,8 @@ Implicit Types x : perm.
 Implicit Types xs : list perm.
 Implicit Types xb : pbit Ti.
 Implicit Types xbs : list (pbit Ti).
+
+Hint Extern 0 (Separation _) => apply (_ : Separation perm).
 
 Lemma pbit_disjoint_valid Γ Γm xb1 xb2 :
   xb1 ⊥ xb2 → ✓{Γ,Γm} xb1 → sep_unmapped xb2 → ✓{Γ,Γm} xb2.
@@ -73,13 +75,30 @@ Lemma pbits_perm_union xbs1 xbs2 :
   tagged_perm <$> xbs1 ∪* xbs2
   = (tagged_perm <$> xbs1) ∪* (tagged_perm <$> xbs2).
 Proof. revert xbs2. induction xbs1; intros [|??]; f_equal'; auto. Qed.
-Lemma PBits_union xs1 xs2 bs :
+Lemma PBits_disjoint xs1 xs2 bs :
+  xs1 ⊥* xs2 →
+  Forall (not ∘ sep_unmapped) xs1 → Forall (not ∘ sep_unmapped) xs2 →
+  zip_with PBit xs1 bs ⊥* zip_with PBit xs2 bs.
+Proof.
+  intros Hxs. revert bs. induction Hxs; intros [|??] ??;
+    decompose_Forall_hyps; constructor; sep_unfold; naive_solver.
+Qed.
+Lemma PBits_union xs1 xs2 (bs : list (bit Ti)) :
+  zip_with PBit (xs1 ∪* xs2) bs = zip_with PBit xs1 bs ∪* zip_with PBit xs2 bs.
+Proof.
+  revert xs2 bs. unfold union at 2, sep_union at 2; simpl.
+  induction xs1; intros [|??] [|??]; f_equal'; simplify_option_equality; auto.
+Qed.
+Lemma PBits_BIndet_union_r xs1 xs2 bs :
   zip_with PBit (xs1 ∪* xs2) bs
   = zip_with PBit xs1 bs ∪* (flip PBit BIndet <$> xs2).
 Proof.
   revert xs2 bs. induction xs1; intros [|??] [|??]; f_equal'; auto.
-  by unfold union at 2,  sep_union at 2; simplify_option_equality.
+  by unfold union at 2, sep_union at 2; simplify_option_equality.
 Qed.
+Lemma PBits_BIndet_disjoint xs1 xs2 :
+  xs1 ⊥* xs2 → (flip PBit (@BIndet Ti) <$> xs1) ⊥* (flip PBit BIndet <$> xs2).
+Proof. induction 1; constructor; sep_unfold; auto. Qed.
 Lemma PBits_BIndet_union xs1 xs2 :
   flip PBit (@BIndet Ti) <$> xs1 ∪* xs2
   = (flip PBit BIndet <$> xs1) ∪* (flip PBit BIndet <$> xs2).
@@ -110,8 +129,40 @@ Proof.
     perm_lock_disjoint, perm_lock_mapped.
   destruct (perm_mapped x1); auto. by transitivity (Some Writable).
 Qed.
+Lemma pbits_lock_disjoint xbs1 xbs2 :
+  Forall (λ xb, Some Writable ⊆ pbit_kind xb) xbs1 →
+  xbs1 ⊥* xbs2 → pbit_lock <$> xbs1 ⊥* xbs2.
+Proof. induction 2; decompose_Forall_hyps; auto using pbit_lock_disjoint. Qed.
 Lemma pbit_lock_union xb1 xb2 : pbit_lock (xb1 ∪ xb2) = pbit_lock xb1 ∪ xb2.
 Proof. sep_unfold. destruct xb1, xb2; f_equal'; auto using perm_lock_union. Qed.
+Lemma pbit_unlock_disjoint xb1 xb2 : xb1 ⊥ xb2 → pbit_unlock xb1 ⊥ xb2.
+Proof.
+  sep_unfold; destruct xb1 as [x1 b1], xb2 as [x2 b2];
+    naive_solver eauto using perm_unlock_disjoint, perm_unlock_unmapped,
+    perm_unlock_mapped, @sep_disjoint_valid_r.
+Qed.
+Lemma pbit_unlock_union xb1 xb2 :
+  xb1 ⊥ xb2 → pbit_locked xb1 → pbit_unlock (xb1 ∪ xb2) = pbit_unlock xb1 ∪ xb2.
+Proof.
+  sep_unfold; intros.
+  destruct xb1, xb2; f_equal'; naive_solver auto using perm_unlock_union.
+Qed.
+Lemma pbits_unlock_disjoint xbs1 xbs2 βs :
+  xbs1 ⊥* xbs2 → βs =.>* pbit_locked <$> xbs1 →
+  zip_with pbit_unlock_if xbs1 βs ⊥* xbs2.
+Proof.
+  rewrite Forall2_fmap_r; intros Hxbs; revert βs; induction Hxbs;
+    intros [|[] ?] ?; decompose_Forall_hyps; auto using pbit_unlock_disjoint.
+Qed.
+Lemma pbits_unlock_union xbs1 xbs2 βs :
+  xbs1 ⊥* xbs2 → βs =.>* pbit_locked <$> xbs1 →
+  zip_with pbit_unlock_if (xbs1 ∪* xbs2) βs
+  = zip_with pbit_unlock_if xbs1 βs ∪* xbs2.
+Proof.
+  rewrite Forall2_fmap_r; intros Hxbs; revert βs; induction Hxbs;
+    intros [|[] ?] ?; decompose_Forall_hyps; f_equal; auto.
+  by apply pbit_unlock_union.
+Qed.
 Lemma pbit_disjoint_full xb1 xb2 :
   xb1 ⊥ xb2 → tagged_perm xb1 = perm_full → xb2 = ∅.
 Proof.
@@ -154,5 +205,41 @@ Lemma pbits_indetified_subseteq xbs1 xbs2 :
 Proof.
   induction 2; simplify_equality';
     f_equal'; eauto using pbit_indetified_subseteq.
+Qed.
+Lemma pbit_union_typed Γ Γm xb1 xb2 :
+  ✓{Γ,Γm} xb1 → ✓{Γ,Γm} xb2 → xb1 ⊥ xb2 → ✓{Γ,Γm} (xb1 ∪ xb2).
+Proof.
+  destruct xb1 as [x1 b1], xb2 as [x2 b2].
+  intros (?&?&?) (?&?&?) (?&?&?&?); simplify_equality'.
+  split; split_ands; sep_unfold; simpl; [case_decide; auto|].
+  split; intros; auto using sep_union_valid.
+  rewrite decide_True by eauto using sep_unmapped_union_l'.
+  eauto using sep_unmapped_union_r'.
+Qed.
+Lemma pbits_union_typed Γ Γm xbs1 xbs2 :
+  ✓{Γ,Γm}* xbs1 → ✓{Γ,Γm}* xbs2 → xbs1 ⊥* xbs2 → ✓{Γ,Γm}* (xbs1 ∪* xbs2).
+Proof. induction 3; decompose_Forall_hyps; auto using pbit_union_typed. Qed.
+Lemma pbit_union_refine Γ α f Γm1 Γm2 xb1 xb2 xb1' xb2' :
+  ✓ Γ → xb1 ⊑{Γ,α,f@Γm1↦Γm2} xb2 → xb1' ⊑{Γ,α,f@Γm1↦Γm2} xb2' →
+  xb2 ⊥ xb2' → xb1 ∪ xb1' ⊑{Γ,α,f@Γm1↦Γm2} xb2 ∪ xb2'.
+Proof.
+  destruct xb1 as [x1 b1], xb2 as [x2 b2], xb1' as [x1' b1'], xb2' as [x2' b2'].
+  intros ? (?&?&[??]&_) (?&?&[??]&_) (?&?&?&?); simplify_equality'.
+  split; split_ands; sep_unfold; simpl; auto.
+  * repeat case_decide;
+      naive_solver eauto 2 using BIndet_refine, bit_refine_valid_r.
+  * split; intros; auto using sep_union_valid.
+    rewrite decide_True by eauto using sep_unmapped_union_l'.
+    eauto using sep_unmapped_union_r'.
+  * split; intros; auto using sep_union_valid.
+    rewrite decide_True by eauto using sep_unmapped_union_l'.
+    eauto using sep_unmapped_union_r'.
+Qed.
+Lemma pbits_union_refine Γ α f Γm1 Γm2 xbs1 xbs2 xbs1' xbs2' :
+  ✓ Γ → xbs1 ⊑{Γ,α,f@Γm1↦Γm2}* xbs2 → xbs1' ⊑{Γ,α,f@Γm1↦Γm2}* xbs2' →
+  xbs2 ⊥* xbs2' → xbs1 ∪* xbs1' ⊑{Γ,α,f@Γm1↦Γm2}* xbs2 ∪* xbs2'.
+Proof.
+  intros ? Hxbs. revert xbs1' xbs2'. induction Hxbs; destruct 1; intros;
+    decompose_Forall_hyps; constructor; auto using pbit_union_refine.
 Qed.
 End permission_bits.
