tactics.v
@@ -219,6 +219,13 @@ Ltac simplify_equality := repeat
   end.
 Ltac simplify_equality' := repeat (progress csimpl in * || simplify_equality).
 Ltac f_equal' := csimpl in *; f_equal.
+Ltac f_lia :=
+  repeat lazymatch goal with
+  | |- @eq BinNums.Z _ _ => lia
+  | |- @eq nat _ _ => lia
+  | |- _ => f_equal
+  end.
+Ltac f_lia' := csimpl in *; f_lia.
 
 (** Given a tactic [tac2] generating a list of terms, [iter tac1 tac2]
 runs [tac x] for each element [x] until [tac x] succeeds. If it does not
